\documentclass[12pt]{article}
\usepackage{fancyhdr}
\usepackage[margin=1 in,headheight=20pt]{geometry}
\usepackage{setspace}
\usepackage{amsmath}
\usepackage{amsthm}
\usepackage{amssymb}
\usepackage{enumerate}
\usepackage{relsize}
\usepackage{lastpage}
\allowdisplaybreaks

\theoremstyle{plain} 
\newtheorem*{thm}{Theorem}

\pagestyle{fancy}
\lhead{COMP 302-001}
\chead{practice-final.ml Induction Proof}
\rhead{\today
	\\ LORE, JULIAN}
\cfoot{Page \thepage \ of \pageref{LastPage}}

\begin{document}
\onehalfspacing
\begin{thm}
  For all trees \texttt{t}, \texttt{size t + acc} $=$ \texttt{size\_acc
  t acc}.
\end{thm}
\begin{proof}
  By structural induction on the depth of \texttt{t}.
  \begin{itemize}
  \item \textbf{Base case}: \texttt{t = Leaf}
    \begin{align*}
      \texttt{size t + acc} &= \texttt{size Leaf + acc} &
      \\ & \Rightarrow
           \texttt{0 + acc} & \text{By definition of \texttt
                        {size}}
      \\ & = \texttt{acc}
      \\ & \Leftarrow \texttt{size\_acc Leaf} & \text{By                           definition of \texttt{size\_acc}}
      \\ & =
           \texttt{size\_acc
           t}
    \end{align*}
  \item \textbf{Step}: \texttt{t} $=$ \texttt{Node(l,x,r)} for some trees
    \texttt{l},\texttt{r} and value \texttt{x}.
    \\ \textbf{Inductive Hypothesis (1)}: \texttt{size l + acc} $=$
    \texttt{size\_acc l acc}, for some tree \texttt{l}
    \\ \textbf{Inductive Hypothesis (2)}: \texttt{size r + acc} $=$
    \texttt{size\_acc r acc}, for some tree \texttt{r}
      \begin{align*}
        & \texttt{size\_acc t acc}
        \\ & = \texttt{size\_acc Node(l,x,r) acc}
        \\ & \Downarrow \texttt{size\_acc l (x + size\_acc r acc)} & \text{By                                                                  definition of                                                                   \texttt{size\_acc}}
        \\ & = \texttt{size l + (x + size\_acc r acc)} & \text{By IH(1)}
        \\ & = \texttt{size l + (x + size r + acc)} & \text{By IH(2)}
        \\ & = \texttt{size l + x + size r + acc} & \text{By               associativity of \texttt{+}}
        \\ & = \texttt{x + size l + size r + acc} & \text{By                 commutativity of \texttt{+}}
        \\ & \Leftarrow \texttt{size Node(l,x,r) + acc} & \text{By definition of \texttt{size}}
        \\ & = \texttt{size t + acc} &
      \end{align*}
  \end{itemize}
\end{proof}
\end{document}