\documentclass[12 pt]{article}
\usepackage{hyperref, fancyhdr, setspace, enumerate, amsmath,
  lastpage, amssymb, algpseudocode, bussproofs, tikz, listings}
\usetikzlibrary{shapes.geometric}
\usetikzlibrary{positioning}
\EnableBpAbbreviations
\usepackage[margin=1 in]{geometry}
\allowdisplaybreaks
%\usepackage[dvipsnames]{xcolor}   %May be necessary if you want to color links
\hypersetup{
	%colorlinks=true, %set true if you want colored links
	linktoc=all,     %set to all if you want both sections and subsections linked
	linkcolor=black,  %choose some color if you want links to stand out
}
\usepackage{graphicx}
\graphicspath{{Images/}}
\author{Julian Lore}
\date{Last updated: \today}
\title{COMP 527: Logic and Computation}
\pagestyle{fancy}
\lhead{COMP 527}
\chead{\leftmark}
\rhead{Julian Lore}
\cfoot{Page \thepage \ of \pageref{LastPage}}
\newcommand{\tab}[1]{\hspace{.2\textwidth}\rlap{#1}}
\newenvironment{rcases}
  {\left.\begin{aligned}}
  {\end{aligned}\right\rbrace}
\begin{document}
	\onehalfspacing
	\maketitle
	\tableofcontents
    \section{01/08/19}
    \paragraph{Goal:}
    \begin{itemize}
    \item Introduction to the proof theoretic foundations
    \item Study the relationship to programming languages and their
      design
    \end{itemize}
    \paragraph{Schedule:}
    \begin{itemize}
    \item Week 1: Natural Deduction
    \item Week 2: Tutorial (Jacob) on using Tutch (proof assistant,
      program on writing Natural Deduction proofs)
    \item Week 3: Proofs in the natural deduction system and programs
      in the $\lambda$-calculus
    \item Week 4: First Order Logic
    \item Week 5: Induction (how we can add induction to logic,
      corresponds to recursion)
    \item Week 6/7: Programming with dependent types
    \item Week 8: Sequent calculus
    \item Week 9: Consistency
    \item Week 10: Proof search
    \item Week 11/12: Linear logic, modal logic or temporal logic
    \end{itemize}
    \subsection{Natural Deduction}
    \begin{itemize}
    \item G. Gentzen started describing it in the mid 30s
    \item Martin L\"of continued in the mid 80s
    \end{itemize}
    \paragraph{Motivation} To design a modular system for
    reasoning. Want to capture the reasoning of mathematicians (that's
    why it's called natural). It is modular because we define the
    meaning of each connective by themselves (will not refer to any
    other connective in the definition).
    \paragraph{Judgment} ``Something we know'' or ``something that is
    evident''
    \\ Ex. $A$ true, ``The proposition $A$ is true'' (Semantics)
    \\ $A$ wf, ``The proposition $A$ is syntactically well-formed''
    (Syntax)
    \\ $A$ true @ $t$, ``The proposition
    $A$ is true at time $t$''
    \\ Can describe both aspects (semantics and syntax) as judgment

    \paragraph{Example Grammar}
    Proposition $A, B:= T \mid \perp \mid A \land B \mid \ldots$
    \begin{prooftree}
      \AXC{}
      \UIC{T wf}
    \end{prooftree}
    \begin{prooftree}
      \AXC{}
      \UIC{$\perp$ wf}
    \end{prooftree}
    \begin{prooftree}
      \AXC{A wf}
      \AXC{B wf}
      \BIC{A $\land$ B wf}
    \end{prooftree}
    \begin{prooftree}
      \AXC{$J_1$ \ldots $J_n$}
      \UIC{$J$}
    \end{prooftree}
    $J_i$ are the premises, $J$ is the conclusion
    \\ $A$ true
    \begin{itemize}
    \item Introduction rules: How can we conclude $A$
    \item Elimination rules: What information can we extract from A?
      (i.e. T, $\perp$, $A \land B$, \ldots)
    \end{itemize}
    \begin{prooftree}
      \AXC{}
      \RL{T I (Introduction)}
      \UIC{T true}
    \end{prooftree}
    No elim rule for T
    \paragraph{Conjunction}
    \begin{prooftree}
      \AXC{A true}
      \AXC{B true}
      \RL{$\land$I}
      \BIC{$A \land B$ true}
    \end{prooftree}
    \begin{prooftree}
      \AXC{$A \land B$ true}
      \RL{$\land$E$_l$ (Elimination)}
      \UIC{$A$ true}
    \end{prooftree}
    \begin{prooftree}
      \AXC{$A \land B$ true}
      \RL{$\land$E$_r$}
      \UIC{$B$ true}
    \end{prooftree}
    What can we now prove?
    \begin{prooftree}
      \AXC{}
      \RL{$T$ I}
      \UIC{$T$ true}
      \AXC{}
      \RL{$T$ I}
      \UIC{$T$ true}
      \RL{$\land$ I}
      \BIC{$T \land T$ true}
    \end{prooftree}
    Is the following a proof?
    \begin{prooftree}
      \AXC{$A \land (B \land C)$ true}
      \RL{$\land$E$_r$}
      \UIC{$B \land C$ true}
      \RL{$\land$ E$_l$}
      \UIC{$B$ true}
    \end{prooftree}
    No, how do we know $A \land (B \land C)$ is true?

    Given the assumption (hypothesis) $A \land (B \land C)$ true, we
    can construct a proof for $B$ true (reasoning by
    assumption/hypothetical reasoning/derivation).
    \begin{prooftree}
      \AXC{}
      \RL{$u_1$}
      \UIC{$J_1$}
      \AXC{\ldots}
      \AXC{}
      \RL{$u_n$}
      \UIC{$J_n$}
      \TIC{\vdots}
      \noLine
      \UIC{$J$}
    \end{prooftree}
    \paragraph{Implication}
    \begin{prooftree}
      \AXC{}
      \RL{$u$}
      \UIC{$A$ true}
      \noLine
      \UIC{\vdots}
      \noLine
      \UIC{$B$ true}
      \RL{$ \supset$ I$^{u}$}
      \UIC{$A \supset B$ true}
    \end{prooftree}
    \begin{prooftree}
      \AXC{$A \supset B$ true}
      \AXC{$A$ true}
      \RL{$\supset$ E}
      \BIC{$B$ true}
    \end{prooftree}
    We do not include $A \supset B$ true, $B$ false, implies $A$
    false, because we did not add a judgment for false, only talking
    about things that are true. If we cannot say something is true, it
    is implied that it is false.

    Let's prove:
    \begin{prooftree}
      \AXC{}
      \RL{$u$}
      \UIC{$A$ true}
      \AXC{}
      \RL{$v$}
      \UIC{$B$ true}
      \RL{$\land$ I}
      \BIC{$A \land B$ true}
      \RL{$\supset I^v$}
      \UIC{$B \supset A \land B$ true}
      \RL{$\supset I^u$}
      \UIC{$A \supset (B\supset A \land B)$ true}
    \end{prooftree}
    \paragraph{Observations}
    \begin{enumerate}
    \item \underline{Order} of assumptions does not matter.
    \item Do I have to use an assumption? No. This is called \underline{weakening}.
      \\ Floating assumption that isn't used:
      \begin{prooftree}
        \AXC{}
        \RL{$v$}
        \UIC{$B$ true}
      \end{prooftree}
      \begin{prooftree}
        \AXC{}
        \RL{$u$}
        \UIC{$A$ true}
        \RL{$\supset I^v$}
        \UIC{$B\supset A$ true}
        \RL{$\supset I^u$}
        \UIC{$A \supset B \supset A$ true}
      \end{prooftree}
    \item Can we use assumptions more than once? Yes. This is called
      \underline{strengthening} (you contract multiple of these
      assumptions into one).
      \begin{prooftree}
        \AXC{}
        \RL{$u$}
        \UIC{$A$ true}
        \AXC{}
        \RL{$u$}
        \UIC{$A$ true}
        \RL{$\land$I}
        \BIC{$A \land A$ true}
        \RL{$\supset I^u$}
        \UIC{$A \supset (A \land A)$ true}
      \end{prooftree}
      This is a program that takes in an input and returns it twice.
    \end{enumerate}
    A simple proof:
    \begin{prooftree}
      \AXC{}
      \RL{$u$}
      \UIC{$A \land B$ true}
      \RL{$\land$ E$_l$}
      \UIC{$A$ true}
      \AXC{}
      \RL{$u$}
      \UIC{$A \land B$ true}
      \RL{$\land$ E$_r$}
      \UIC{$B$ true}
      \RL{$\land$I}
      \BIC{$B\land A$ true}
      \RL{$\supset I^u$}
      \UIC{$(A \land B) \supset (B \land A)$ true}
    \end{prooftree}
    \section{01/10/18}
    \subsection{Natural Deduction}
    \underline{A true}
    \paragraph{Conjunction}
    \begin{prooftree}
      \AXC{$A$ true}
      \AXC{$B$ true}
      \RL{$\land$ I}
      \BIC{$A \land B$ true}
    \end{prooftree}
    \begin{prooftree}
      \AXC{$A \land B$ true}
      \RL{$\land$E$_l$ (Elimination)}
      \UIC{$A$ true}
    \end{prooftree}
    \begin{prooftree}
      \AXC{$A \land B$ true}
      \RL{$\land$E$_r$}
      \UIC{$B$ true}
    \end{prooftree}
    \paragraph{Implications}
    This discharges the assumption $u$ and is the only rule we have
    right now that discharges assumptions.
    \begin{prooftree}
      \AXC{}
      \RL{$u$}
      \UIC{$A$ true}
      \noLine
      \UIC{\vdots}
      \noLine
      \UIC{$B$ true}
      \RL{$ \supset$ I$^{u}$}
      \UIC{$A \supset B$ true}
    \end{prooftree}
    \begin{prooftree}
      \AXC{$A \supset B$ true}
      \AXC{$A$ true}
      \RL{$\supset$ E}
      \BIC{$B$ true}
    \end{prooftree}
    \paragraph{Truth}
    \begin{prooftree}
      \AXC{}
      \RL{T I}
      \UIC{T true}
    \end{prooftree}
    To get the smallest complete example, we need to introduce
    $\perp$.
    \paragraph{Falsehood}
    No Intro-Rule for $\perp$.
    \begin{prooftree}
      \AXC{$\perp$ true}
      \RL{$\perp$ E}
      \UIC{$A$ true}
    \end{prooftree}
    Define Negation as an abbreviation (notational definition)
    $$\neg A \equiv A \supset \perp$$
    \begin{prooftree}
      \AXC{}
      \RL{u}
      \UIC{$A \land \neg A$}
      \RL{$\land$ E$_l$}
      \UIC{$A$}
      \AXC{}
      \RL{u}
      \UIC{$A \land \neg A$}
      \RL{$\land$ E$_r$}
      \UIC{$\neg A \equiv (A \supset \perp)$}
      \RL{$\supset$ E}
      \BIC{$\perp$}
      \RL{$\supset$ I$^u$}
      \UIC{$\neg (A \land \neg A)$ true}
    \end{prooftree}
    If we could prove $\perp$ from no assumptions, then our system
    would be inconsistent.
    \paragraph{Examples}
    \begin{prooftree}
      \AXC{}
      \RL{u}
      \UIC{$A\supset (B \land C)$ true}
      \AXC{}
      \RL{v}
      \UIC{$A$ true}
      \RL{$\supset$ E}
      \BIC{$B \land C$ true}
      \RL{$\land$ E$_l$}
      \UIC{$B$ true}
      \RL{$\supset$I$^v$}
      \UIC{$A \supset B$ true}
      \AXC{}
      \RL{u}
      \UIC{$A \supset (B \land C)$ true}
      \AXC{}
      \RL{v}
      \UIC{$A$ true}
      \BIC{$B \land C$}
      \RL{$\land$ E}
      \UIC{$C$ true}
      \RL{$\supset$ I$^v$}
      \UIC{$A \supset C$ true}
      \RL{$\land$ I}
      \BIC{$(A \supset B) \land (A \supset C)$ true}
      \RL{$\supset$ I$^u$}
      \UIC{$(A \supset (B \land C)) \supset ((A \supset B) \land
        (A \supset C)) = (A \land \neg A) \supset \perp$ true}
    \end{prooftree}
    Note that the assumptions u and v are used twice, but in different
    areas.
    \begin{prooftree}
      \AXC{}
      \RL{u}
      \UIC{$A$}
      \AXC{}
      \RL{v}
      \UIC{$\neg A$}
      \RL{$\supset$ E}
      \BIC{$\perp$}
      \RL{$\supset$ I$^v$}
      \UIC{$\neg \neg A = \neg A \supset \perp$ true}
      \RL{$\supset$ I$^u$}
      \UIC{$A \supset \neg \neg A$ true}
    \end{prooftree}
    Is $A = \neg \neg A$? We cannot prove this in this logic unless we
    assume an axiom (although it is true for classical logic).

    For a proof, we must discharge all assumptions we make.

    \paragraph{Local Soundness}
    How do we know the rules we defined for natural deduction make
    sense?

    Elimination Rules are not too strong (they don't allow us to
    conclude more than we should be able to). If the rules are too
    strong, we'll be able to prove things that we shouldn't be able
    to, more than we had to start with.

    Given a proof $\mathcal{D}$ for $A$ true and a proof $\mathcal{E}$ for
    $B$ true, we can prove $A$ true.
    \begin{center}
      \AXC{$\mathcal{D}$}
      \noLine
      \UIC{$A$ true}
      \AXC{$\mathcal{E}$}
      \noLine
      \UIC{$B$ true}
      \RL{$\land$ I}
      \BIC{$A \land B$ true}
      \RL{$\land$ E}
      \UIC{$A$ true}
      \DP
      $\implies$
      \begin{tabular}{c}
      $\mathcal{D}$
      \\ $A$ true
      \end{tabular}
    \end{center}
    \begin{center}
      \AXC{$\mathcal{D}$}
      \noLine
      \UIC{$A$ true}
      \AXC{$\mathcal{E}$}
      \noLine
      \UIC{$B$ true}
      \RL{$\land$ I}
      \BIC{$A \land B$ true}
      \RL{$\land$ E}
      \UIC{$B$ true}
      \DP
      $\implies$
    \begin{tabular}{c}
      $\mathcal{E}$\\ $B$ true
    \end{tabular}
    \end{center}
    \paragraph{Local Completeness}
    Elimination Rules are not too weak, i.e. we are expanding proofs.
    \begin{center}
    \begin{tabular}{c}
      $\mathcal{D}$ \\ $A \land B$ true 
    \end{tabular}
    $\implies$
    \AXC{$\mathcal{D}$}
    \noLine
    \UIC{$A \land B$ true}
    \RL{$\land$ E$_l$}
    \UIC{$A$ true}
    \AXC{$\mathcal{D}$}
    \noLine
    \UIC{$A \land B$ true}
    \RL{$\land$ E$_r$}
    \UIC{$B$ true}
    \RL{$\land$ I}
    \BIC{$A \land B$ true}
    \DP
    \end{center}
    \paragraph{Local Soundness (Implication)}
    \begin{center}
    \AXC{}
      \RL{u}
      \UIC{$A$ true}
      \noLine
      \UIC{\vdots}
      \noLine
      \UIC{$\mathcal{D}^u$}
      \noLine
      \UIC{$B$ true}
      \RL{$\supset$ I$^u$}
      \UIC{$A \supset B$ true}
      \AXC{$\mathcal{E}$}
      \noLine
      \UIC{$A$ true}
      \RL{$\supset$ E}
      \BIC{$B$ true}
      \DP
      $\implies$
      \begin{tabular}{c}
        $\mathcal{E}$
        \\$A$ true
      \\$[\mathcal{E}/u] (\mathcal{D})$
      \\$B$ true 
      \end{tabular}
    \end{center}
    \paragraph{Substitution Principle}
    \begin{center}
    If
      \AXC{}
      \RL{u}
      \UIC{$A$ true}
      \noLine
      \UIC{$\vdots$}
      \noLine
      \UIC{$\mathcal{D}$}
      \noLine
      \UIC{$B$ true}
      \DP
      and
      \begin{tabular}{c}
        \begin{tikzpicture} [
          triangle/.style = {fill=blue!20, regular polygon, regular polygon sides=3 },
          node rotated/.style = {rotate=180},
          border rotated/.style = {shape border rotate=180}
          ]
          \node[triangle, border rotated] {$\mathcal{E}$};
        \end{tikzpicture}\\
        $A$ true 
      \end{tabular},
      then
      \begin{tabular}{c}
        \begin{tikzpicture} [
          triangle/.style = {fill=blue!20, regular polygon, regular polygon sides=3 },
          node rotated/.style = {rotate=180},
          border rotated/.style = {shape border rotate=180}
          ]
          \node[triangle, border rotated] {$\mathcal{E}$};
        \end{tikzpicture}\\
    $A$ true \\ $\mathcal{D}$ \\ $B$ true
      \end{tabular}
    \end{center}

    Basically, if we have a proof for $A$ true and from $A$ true we
    can show $B$ true, then we have a proof for $B$ true.

    \paragraph{Local Completeness}
    \begin{center}
      \begin{tabular}{c}
        $\alpha$
        \\$A \supset B$ true
      \end{tabular}
      $\implies$
      \AXC{$\alpha$}
      \noLine
      \UIC{$A \supset B$ true}
      \AXC{}
      \RL{u}
      \UIC{$A$ true}
      \RL{$\supset$ E}
      \BIC{$B$ true}
      \RL{$\supset$ I$^u$}
      \UIC{$A \supset B$ true}
      \DP
    \end{center}
    So we can prove $A \supset B$ from $A \supset B$.

    Another form of $\land$ elimination:
    \begin{prooftree}
      \AXC{$A \land B$ true}
      \AXC{}
      \RL{u}
      \UIC{$A$ true}
      \AXC{}
      \RL{v}
      \UIC{$B$ true}
      \noLine
      \BIC{\vdots}
      \noLine
      \UIC{$C$ true}
      \RL{$\land E^{u,v}$}
      \BIC{$C$ true}
    \end{prooftree}
    We could use this new rule and check for local soundness and
    completeness like above.

    Could have unused, floating assumption:
    \begin{prooftree}
      \AXC{}
      \RL{a}
      \UIC{$A$ true}
    \end{prooftree}
    \begin{prooftree}
      \AXC{}
      \RL{u}
      \UIC{$A \land B$}
      \RL{b}
      \UIC{$B$ true}
      \AXC{\vdots}
      \noLine
      \UIC{$A$ true}
      \BIC{$B \land A$ true}
      \RL{$\supset$ I$^u$}
      \UIC{$A \land B \supset B \land A$ true}
    \end{prooftree}
    \subsection{Disjunction}
    Intro-Rules:
    \begin{prooftree}
      \AXC{$A$ true}
      \RL{$\lor$ I$_l$}
      \UIC{$A \lor B$ true}
    \end{prooftree}
    \begin{prooftree}
      \AXC{$B$ true}
      \RL{$\lor$ I$_r$}
      \UIC{$A \lor B$ true}
    \end{prooftree}
    Might be tempted to make the following rule:
    \begin{prooftree}
      \AXC{$B$ true}
      \RL{$\lor$ I$_r$}
      \UIC{$A \lor B$ true}
      \RL{?}
      \UIC{$A$ true}
    \end{prooftree}
    This is locally unsound! Got information we didn't start with.

    We also cannot introduce:
    \begin{prooftree}
      \AXC{$A \lor B$}
      \UIC{$\neg A \supset B$ true}
    \end{prooftree}
    This violates our principle of modularity, as we don't want to
    refer to a different kind of connective.

    Our elimination rule:
    \begin{prooftree}
      \AXC{$A \lor B$ true}
      \AXC{}
      \RL{u}
      \UIC{$A$ true}
      \noLine
      \UIC{\vdots}
      \noLine
      \UIC{$C$ true}
      \AXC{}
      \RL{v}
      \UIC{$B$ true}
      \noLine
      \UIC{\vdots}
      \noLine
      \UIC{$C$ true}
      \RL{$\lor$ E$^{u,v}$}
      \TIC{$C$ true}
    \end{prooftree}
    \paragraph{Example}
    \begin{prooftree}
      \AXC{}
      \RL{u}
      \UIC{$A \lor (B \land C)$ true}
      \AXC{}
      \RL{a}
      \UIC{$A$ true}
      \RL{$\lor$ I$_l$}
      \UIC{$A \lor C$ true}
      \AXC{}
      \RL{b}
      \UIC{$B \land C$ true}
      \RL{$\land$ E$_l$}
      \UIC{$A \lor B$ true}
      \UIC{$B$ true}
      \RL{$\lor$ I$_r$}
      \RL{$\lor$ E}
      \TIC{$A \lor B$ true}
      \AXC{\vdots}
      \noLine
      \UIC{$A \lor C$ true} % Same proof as other thing (almost)
      \RL{$\lor$ I}
      \BIC{$(A \lor B)\land (A \lor C)$}
      \RL{$\supset$ I}
      \UIC{$(A \lor (B \land C))\supset (A \lor B)\land (A \lor C)$}
    \end{prooftree}
    \section{01/15/19}
    Recall: We defined $\neg A$ as $A \supset \perp$. But, there are
    other ways you can introduce (define) negation.
    \subsection{Negation}
    \begin{prooftree}
      \AXC{}
      \RL{u}
      \UIC{$A$ true}
      \noLine
      \UIC{\vdots}
      \noLine
      \UIC{$p$ true}
      \RL{$\neg$ I$^{u,p}$}
      \UIC{$\neg A$ true}
    \end{prooftree}
    If we can prove any parameter $p$ from $A$ true, then $\neg A$ is
    true. This discharges the assumption $u$ and $p$.
    \begin{prooftree}
      \AXC{$\neg A$ true}
      \AXC{$A$ true}
      \RL{$\neg$ E}
      \BIC{$C$ true}
    \end{prooftree}
    For these new rules, as usual, we want to prove that they are
    locally sound and complete. In general, for local soundness, you
    want to introduce the rule and then eliminate it and show that
    you've learned nothing new.
    \paragraph{Local Soundness}
    \begin{center}
      \AXC{}
      \RL{u}
      \UIC{$A$ true}
      \noLine
      \UIC{$D$}
      \noLine
      \UIC{$p$ true}
      \RL{$\neg$ I$^{p,u}$}
      \UIC{$\neg A$ true}
      \AXC{$\mathcal{E}$}
      \noLine
      \UIC{$A$ true}
      \RL{$\neg$ E}
      \BIC{$C$ true}
      \DP
      $\implies$
      \begin{tabular}{c}
        $ [\mathcal{E}/u, C/p]D$
        \\ $C$ true
      \end{tabular}
    \end{center}
    \paragraph{Local Completeness}
    For local completeness, we want to introduce a pointless detour,
    i.e. introduce the rule and then get rid of it and show that we
    haven't affected the proof.
    \begin{center}
      \begin{tabular}{c}
        $\mathcal{D}$
        \\ $\neg A$ true
      \end{tabular}
      $\implies$
      \AXC{$\mathcal{D}$}
      \noLine
      \UIC{$\neg A$ true}
      \AXC{}
      \RL{u}
      \UIC{$A$ true}
      \RL{$\neg$ E}
      \BIC{$p$ true}
      \RL{$\neg$ I$^{p,u}$}
      \UIC{$\neg A$ true}
      \DP
    \end{center}
    \subsection{Classical Reasoning}
    Basic idea behind proof by contradiction, you assume $\neg A$,
    arrive at a contradiction and then you can prove $A$ true.

    \begin{prooftree}
      \AXC{}
      \RL{u}
      \UIC{$\neg A$ true}
      \noLine
      \UIC{\vdots}
      \noLine
      \UIC{$p$ true}
      \RL{$C^{u,p}$}
      \UIC{$A$ true}
    \end{prooftree}
    where $C^{u,p}$ means a proof by contradiction under $u$ and $p$.
    \paragraph{Law of Excluded Middle}
    Want to show $\neg A \lor A$ is true for all $A$.
    \begin{prooftree}
      
      \AXC{}
      \RL{u}
      \UIC{$\neg (\neg A \lor A)$ true}

      \AXC{}
      \RL{v}
      \UIC{$\neg A$}
      \RL{$\lor$ I$_l$}
      \UIC{$\neg A \lor A$}
      
      \RL{$\neg$ E}
      \BIC{$p$ true}
      \RL{$C^{v,p}$}
      \UIC{$A$}
      \RL{$\lor$ I$_r$}
      \UIC{$\neg A \lor A$}
      
      \AXC{}
      \RL{u}
      \UIC{$\neg (\neg A \lor A)$ true}
      \RL{$\neg$ E}
      
      \BIC{$q$ true}
      \RL{$C^{u,q}$}
      \UIC{$\neg A \lor A$}
    \end{prooftree}
    \paragraph{Law of Excluded Middle and more examples in tutch}
    \lstinputlisting{lem.tut}
    \subparagraph{Output}
    \lstinputlisting{lem.tut.output}
    \subsection{NAND}
    $A \overline{\land} B \equiv \neg (A \land B)$

    Showing this introduction rule is often a midterm question. Often,
    people make the mistake of using $A \land B$, but we cannot
    introduce other connectives, make sure $A$ and $B$ are separate.
    \begin{prooftree}
      \AXC{}
      \RL{u}
      \UIC{$A$ true}
      \AXC{}
      \RL{v}
      \UIC{$B$ true}
      \noLine
      \BIC{\vdots}
      \noLine
      \UIC{$p$ true}
      \RL{$\overline{\land}$ I}
      \UIC{$A \overline{\land} B$ true}
    \end{prooftree}
    \begin{prooftree}
      \AXC{$A$ true}
      \AXC{$B$ true}
      \AXC{$A \overline{\land} B$ true}
      \RL{$\overline{\land}$ E}
      \TIC{$C$ true}
    \end{prooftree}
    \paragraph{Local Soundness}
    Get rid of assumptions by substituting $\mathcal{E}_1,
    \mathcal{E}_2$ and $C$ into $\mathcal{D}$.
    \begin{center}
      \AXC{}
      \RL{u}
      \UIC{$A$ true}
      \AXC{}
      \RL{v}
      \UIC{$B$ true}
      \noLine
      \BIC{$\mathcal{D}$}
      \noLine
      \UIC{$p$ true}
      \RL{$\overline{\land}$ I$^{u,v,p}$}
      \UIC{$A \overline{\land} B$ true}
      \AXC{$\mathcal{E}_1$}
      \noLine
      \UIC{$A$ true}
      \AXC{$\mathcal{E}_2$}
      \noLine
      \UIC{$B$ true}
      \TIC{$C$ true}
      \DP
      $\implies$
      \begin{tabular}{c}
        $[\mathcal{E}_1/u, \mathcal{E}_2/v, C/p] \mathcal{D}$
        \\ $C$ true
      \end{tabular}
    \end{center}
    \paragraph{Local Completeness}
    \begin{center}
      \begin{tabular}{c}
        $\mathcal{D}$
        \\ $A \overline{\land} B$
      \end{tabular}
      $\implies$
      \AXC{}
      \RL{u}
      \UIC{$A$ true}
      \AXC{}
      \RL{v}
      \UIC{$B$ true}
      \AXC{$\mathcal{D}$}
      \noLine
      \UIC{$A \overline{\land} B$ true}
      \RL{$\overline{\land}$ E}
      \TIC{$p$ true}
      \RL{$\overline{\land}$ I$^{u,v,p}$}
      \UIC{$A \overline{\land} B$}
      \DP
    \end{center}
    Look for other connectives and do these proofs, as they will
    probably be on the midterm.
    \section{01/17/19}
    \subsection{Context}
    So we've seen several rules so far:
    \begin{prooftree}
      \AXC{}
      \UIC{$T$ true}
    \end{prooftree}
    \begin{prooftree}
      \AXC{$\perp$ true}
      \RL{}
      \UIC{$C$ true}
    \end{prooftree}
    \begin{prooftree}
      \AXC{$A$ true}
      \AXC{$B$ true}
      \RL{$\land$ I}
      \BIC{$A \land B$}
    \end{prooftree}
    \begin{prooftree}
      \AXC{$A \land B$ true}
      \RL{$\land$ E$_l$}
      \UIC{$A$ true}
    \end{prooftree}
    \begin{prooftree}
      \AXC{$A \lor B$ true}
      \AXC{}
      \RL{u}
      \UIC{$A$ true}
      \noLine{}
      \UIC{\vdots}
      \noLine
      \UIC{$C$ true}
      
      \AXC{}
      \RL{v}
      \UIC{$B$}
      \noLine
      \UIC{$\vdots$}
      \noLine
      \UIC{$C$ true}
      \RL{$\lor$ E$^{u,v}$}
      \TIC{$C$ true}
    \end{prooftree}
    We are now going to extend these rules with contexts, which allows
    us to know what we've proved and what assumptions we have at each
    step.

    Instead of $A$ true, we will write $\Gamma \vdash A$ true. This
    means:

    ``A is true in context $\Gamma$.''

    $$\Gamma ::= \cdot \mid \Gamma, u:A \text{ true}$$

    So:
    \begin{center}
      \AXC{}
      \RL{u}
      \UIC{$A$ true}
      \noLine
      \UIC{\vdots}
      \noLine
      \UIC{$B$ true}
      \RL{$\supset$ I$^u$}
      \UIC{$A \supset B$ true}
      \DP
      $\stackrel{+\Gamma}{\longrightarrow}$
      \AXC{$\Gamma,u:A$ true $\vdash B$ true}
      \UIC{$\Gamma \vdash A \supset B$ true}
      \DP
    \end{center}
    \begin{prooftree}
      \AXC{}
      \UIC{$\Gamma \vdash T$ true}
    \end{prooftree}
    \begin{prooftree}
      \AXC{$\Gamma \vdash \perp$ true}
      \RL{}
      \UIC{$\Gamma \vdash C$ true}
    \end{prooftree}
    \begin{prooftree}
      \AXC{$\Gamma \vdash A$ true}
      \AXC{$\Gamma \vdash B$ true}
      \RL{$\land$ I}
      \BIC{$\Gamma \vdash A \land B$}
    \end{prooftree}
    \begin{prooftree}
      \AXC{$\Gamma \vdash A \land B$ true}
      \RL{$\land$ E$_l$}
      \UIC{$\Gamma \vdash A$ true}
    \end{prooftree}
    \begin{prooftree}
      \AXC{$\Gamma \vdash A \lor B$ true}
      \AXC{$\Gamma,u: A $ true $\vdash C$}
      \AXC{$\Gamma,v: B $ true $\vdash C$}
      \RL{$\lor$ E$^{u,v}$}
      \TIC{$\Gamma\vdash C$ true}
    \end{prooftree}
    For something to be derived from a context:
    \begin{prooftree}
      \AXC{$u: A$ true $\in \Gamma$}
      \RL{H}
      \UIC{$\Gamma \vdash A$ true}
    \end{prooftree}
    \paragraph{Example}
    \begin{prooftree}
      \AXC{$A \in \Gamma, A, B$}
      \RL{H}
      \UIC{$\Gamma, A, B \vdash$ A}
      \AXC{$B \in \Gamma, A, B$}
      \RL{$H$}
      \UIC{$\Gamma, A, B \vdash$ B}
      
      \RL{$\land$ I}
      \BIC{$\Gamma, u: A$ true, $B$ true $\vdash A \land B$}
      \RL{$\supset$ I}
      \UIC{$\Gamma,u:A$ true $\vdash B \supset A \land B$}
      \RL{$\supset$ I}
      \UIC{$\Gamma \vdash A \supset B \supset A \land B$}
    \end{prooftree}
    \subsection{The Curry-Howard Correspondence}
    We can see that natural deduction is the same as
    functional programming:
    \\
    \begin{tabular}{c c}
      Logic & Types
      \\ \hline $\perp$ & unit
      \\ $A \land B$ & $A \times B$
      \\ $A \lor B$ & $A + B$
      \\ $A \supset B$ & $A \implies B$
      \\ $\perp$ & $\emptyset$
      \\ proofs & programs
      \\ checking a proof & type checker
    \end{tabular}
    \\
    
    $\emptyset$ is the empty type. There is no proof for $\perp$,
    which is why there is no program for $\emptyset$, the two sides
    are equivalent.

    Proof terms capture the structure of a derivation.

    \begin{prooftree}
      \AXC{}
      \RL{H}
      \UIC{$\Gamma,x:A,y:B\vdash x:A$}
      \AXC{}
      \RL{H}
      \UIC{$\Gamma,x:A,y:B\vdash y:B$}
      \RL{$\times$ I}
      \BIC{$\Gamma,x:A,y:B \vdash (x,y): A \times B$}
      \RL{$\implies$ I$^y$}
      \UIC{$\Gamma,x:A \vdash fn\ y \implies (x,y): B \implies A \times
        B$}
      \RL{$\implies$ I$^x$}
      \UIC{$\Gamma \vdash fn\ x \implies fn\ y \implies (x,y) : A \implies B \implies A \times B$}
    \end{prooftree}

    $\Gamma \vdash M : A$ means:\\
    ``M is a proof term (program) for proposition (of type) A.''
    \subsection{Proof Terms}
    Let's upgrade the rules we mentioned earlier to types:
    \begin{prooftree}
      \AXC{}
      \UIC{$\Gamma \vdash () : unit$}
    \end{prooftree}
    \begin{prooftree}
      \AXC{$\Gamma \vdash M: \emptyset$}
      \RL{}
      \UIC{$\Gamma \vdash abort\ M : C$}
    \end{prooftree}
    \begin{prooftree}
      \AXC{$\Gamma \vdash M_1: A$ true}
      \AXC{$\Gamma \vdash M_2: B$ true}
      \RL{$\times$ I}
      \BIC{$\Gamma \vdash (M_1, M_2)\ A\ B$ true}
    \end{prooftree}
    \begin{prooftree}
      \AXC{$\Gamma \vdash M: A \times B$}
      \RL{$\times$ E$_l$}
      \UIC{$\Gamma \vdash fst\ M: A$}
    \end{prooftree}
    \begin{prooftree}
      \AXC{$\Gamma \vdash M: A \times B$}
      \RL{$\times$ E$_r$}
      \UIC{$\Gamma \vdash snd\ M: B$}
    \end{prooftree}
    \begin{prooftree}
      \AXC{$\Gamma \vdash M: A + B$ true}
      \AXC{$\Gamma,u: A \vdash N_1:C$}
      \AXC{$\Gamma,v: B \vdash N_2:C$}
      \RL{$+$ E}
      \TIC{$\Gamma\vdash $ case $M$ of}
      \noLine
      \UIC{inl $u \implies N_1$}
      \noLine
      \UIC{inr $v \implies N_2$}
    \end{prooftree}
    (Where inl is inject left and inr is inject right) Note that this
    is pattern matching!
    \begin{prooftree}
      \AXC{$\Gamma, x:A \vdash M:B$}
      \UIC{$\Gamma \vdash (fn\ x \implies M):A \implies B$}
    \end{prooftree}
    \begin{prooftree}
      \AXC{$\Gamma \vdash M : A$}
      \RL{$+$ I$_l$}
      \UIC{$\Gamma \vdash inl \ M: A + B$}
    \end{prooftree}
    \begin{prooftree}
      \AXC{$\Gamma \vdash M : B$}
      \RL{$+$ I$_r$}
      \UIC{$\Gamma \vdash inr \ M: A + B$}
    \end{prooftree}
    \begin{prooftree}
      \AXC{$\Gamma \vdash M : A \implies B$}
      \AXC{$\Gamma \vdash N : A$}
      \BIC{$\Gamma \vdash M\_N: B$}
    \end{prooftree}
    where $\_$ is a space.
    \paragraph{Example}
    We did this on Tuesday, now we'll see it with proof terms.
    \begin{prooftree}
      \AXC{}
      \RL{H}
      \UIC{$\Gamma, x : A \times B \vdash x : A \times B$}
      \RL{$\times$ E}
      \UIC{$\Gamma, x: A \times B \vdash snd\ x : B$}
      
      \AXC{}
      \RL{H}
      \UIC{$\Gamma, x : A \times B \vdash x : A \times B$}
      \RL{$\times$ E}
      \UIC{$\Gamma, x: A \times B \vdash fst\ x : A$}
      \RL{$\times$ I}
      
      \BIC{$\Gamma, x: A \times B \vdash (snd\ x, fst\ x) : B \times
        A$}
      \RL{$\implies$ I}
      \UIC{$\Gamma \vdash fn\ x \implies (snd\ x, fst\ x) : A \times B \implies B \times A$}
    \end{prooftree}
    \paragraph{Tutch Examples}
    \lstinputlisting[breaklines=true]{proofterms.tut}
    \section{01/22/19}
    \subsection{Metatheory}
    Proving things (properties) about a given theory, this will
    eventually lead us to completeness.

    So far, we've seen:
    \paragraph{Propositions/Types} $A,B:=T \mid \perp \mid A \supset B \mid A
    \land B \mid A \lor B$

    \paragraph{Proof Terms} $M,N := \langle \rangle \mid abort^{A}\ M
    \mid \underbrace{\lambda x: A.M}_{fn\ x \implies M} \mid M \ N$

    \begin{prooftree}
      \AXC{$M : \perp$}
      \UIC{$abort^{A}\ M : A$}
    \end{prooftree}

    Note that: $M : A$ means: Term $M$ has type $A$ or $M$ is a proof
    witness for the proposition $A$

    Types that have one type are sometimes just called singleton
    types.

    Earlier we saw:
    \begin{prooftree}
      \AXC{}
      \RL{$u_1$}
      \UIC{$A_1$ true}
      \UIC{$\ddots$}

      \AXC{\ldots}

      \AXC{}
      \RL{$u_n$}
      \UIC{$A_n$ true}
      \UIC{$\ddots$}

      \TIC{$C$ true}
    \end{prooftree}
    More compactly: Context $\Gamma := \cdot \mid T, A$ true

    $$\Gamma \underbrace{\vdash}_{\text{turnstyle}} C \text{ true}$$

    \paragraph{Reminder about Contexts}
    Context $\Gamma := \cdot \mid \Gamma, x: A$
    \begin{prooftree}
      \AXC{$\Gamma \vdash M : \perp$}
      \UIC{$\Gamma \vdash abort^{A}\ M : A$}
    \end{prooftree}
    \begin{prooftree}
      \AXC{$\Gamma,x:A \vdash M : B$}
      \UIC{$\Gamma \vdash \lambda x:A.M: A \supset B$}
    \end{prooftree}
    \begin{prooftree}
      \AXC{$\Gamma \vdash M : A \supset B$}
      \AXC{$\Gamma \vdash N : A$}
      \BIC{$\Gamma \vdash M\ N:B$}
    \end{prooftree}
    \begin{prooftree}
      \AXC{$x : A \in \Gamma$}
      \UIC{$\Gamma \vdash x : A$}
    \end{prooftree}
    \begin{prooftree}
      \AXC{$\Gamma \vdash M : A$}
      \AXC{$\Gamma \vdash N : B$}
      \BIC{$\Gamma \vdash \langle M, N \rangle : A \land B$}
    \end{prooftree}
    \begin{prooftree}
      \AXC{$\Gamma \vdash M : A \land B$}
      \UIC{$\Gamma \vdash fst \ M : A$}
    \end{prooftree}
    Note that, some may be inclined to make $A \land B$ have a type of
    some pair, like $(M,N)$, but we don't want to limit ourselves to a
    pair (we also don't yet know it's a pair), so we cannot make it a
    pair right off the bat.
    \begin{prooftree}
      \AXC{$\Gamma \vdash M : A \land B$}
      \UIC{$\Gamma \vdash snd \ M : B$}
    \end{prooftree}
    What would we like to compute with these rules?

    General form: $M \implies M'$, Term $M$ reduces to $M'$.
    \\ $fst\ \langle M, N \rangle \implies M$
    \\ $snd\ \langle M, N \rangle \implies N$

    So we can now show things like local soundness:
    \begin{center}
      \AXC{$\mathcal{D}_1$}
      \noLine
      \UIC{$\Gamma \vdash M : A$}
      \AXC{$\mathcal{D}_2$}
      \noLine
      \UIC{$\Gamma \vdash N : B$}
      \RL{$\land$ I}
      \BIC{$\Gamma \vdash \langle M, N \rangle : A \land B$}
      \RL{$\land$ E$_l$}
      \UIC{$\Gamma \vdash fst \ \langle M, N \rangle : A$}`
      \DP
      $\implies$
      \begin{tabular}{c}
        $\mathcal{D}_1$
        \\ $M : A$
      \end{tabular}
    \end{center}
    Local Soundness here corresponds to Subject Reduction/Type
    Preservation.

    We've essentially proved that if we start with something well
    typed (of type $A$), we end up with something that is still well
    typed, we can show that our program is type \textbf{safe}.

    Now if we have a function:

    $(\lambda x : A . M) N \implies [N/x] M$
    \paragraph{Simple Program}
    \begin{align*}
      & fst \ ((\lambda x . \lambda y . \langle x , y \rangle) \langle \rangle \langle \rangle)
      \\ \implies & fst \ \langle \langle \rangle, \langle \rangle \rangle
      \\ \implies & \langle \rangle : T
    \end{align*}
    The type of this program is unit, because we have stated earlier
    that the type we start with is the type we end with. How do we
    know the first line is of type unit?
    \begin{prooftree}

      \AXC{}
      \RL{var}
      \UIC{$x:T, y:T \vdash x:T$}
      
      \AXC{}
      \RL{var}
      \UIC{$x:T, y:T \vdash y:T$}

      \RL{$\land$ I}
      \BIC{$x: T, y:T \vdash \langle x,y \rangle : T \land T$}
      \UIC{$x:T \vdash \lambda y:T \langle x,y \rangle : T \supset (T
        \land T)$}
      \RL{$\supset$ I}
      \UIC{$\lambda x: T \lambda . y: T \langle x,y \rangle : T \supset
        T \supset (T \land T)$}
      
      \AXC{}
      \RL{$T$ I}
      \UIC{$\langle \rangle$ : T}
      
      \RL{$\supset$ E}
      \BIC{$(\lambda x : T \lambda . y: T \langle x,y \rangle)$ : $\langle \rangle$}
      
      \AXC{}
      \RL{$T$ I}
      \UIC{$\langle \rangle$ : T}
      
      \BIC{$((\lambda x:T . \lambda y: T \langle x,y \rangle) \langle
        \rangle) \langle \rangle$ : }
      \RL{$\land$ E$_l$}
      \UIC{$fst\ (\lambda x : T . \lambda y : T \langle x,y \rangle)
        \langle \rangle \langle \rangle$ : }
    \end{prooftree}

    The following is a theorem we are not going to prove:

    If $\Gamma \vdash M : A$ and $M \implies M'$ then $\Gamma \vdash
    M': A$
    
    If $\Gamma \vdash M' : A$ and $M \implies M'$ then $\Gamma \vdash
    M: A$
    \subsection{Congruence Rules}
    We can go into functions. This strategy is non-deterministic (will
    this terminate? Yes, but it is not obvious how to prove it. This
    is a metatheoretic property)
    \begin{prooftree}
      \AXC{$M \implies M'$}
      \UIC{$fst \ M \implies fst \ M'$}
    \end{prooftree}
    \begin{prooftree}
      \AXC{$M \implies M'$}
      \UIC{$snd \ M \implies snd \ M'$}
    \end{prooftree}
    \begin{prooftree}
      \AXC{$M \implies M'$}
      \UIC{$M \ N \implies M' \ N$}
    \end{prooftree}
    \begin{prooftree}
      \AXC{$N \implies N'$}
      \UIC{$M \ N \implies M \ N'$}
    \end{prooftree}
    \begin{prooftree}
      \AXC{$M \implies M'$}
      \UIC{$\lambda x:A.M \implies \lambda x : A.M'$}
    \end{prooftree}
    \paragraph{Syntactic Equality} is important because we want to
    introduce substitution.
    \\\begin{tabular}{l l}
      $\lambda x.x = \lambda y.y$ & \text{(the name of a bound var
                                  does not matter)}
        \\ $\lambda x . \lambda y. x \neq \lambda x . \lambda y . y$
        \\ $\lambda x. \lambda y. x = \lambda x' . \lambda y . x'$ & These are the same because $x$ has the same binding site as $x'$
      \end{tabular}
      \\
    Terms that only differ in the names of the bound variables are
    considered equal. This is defined as
    $\alpha$-renaming. Capture-avoiding substitution.

    Note in the following expression, $x$ is new (``fresh''). We
    cannot have two variables with the same name, if this was the
    case, we'd have to rename $x$. 

    \begin{prooftree}
      \AXC{$\Gamma, x: A \vdash M : B$}
      \UIC{$\Gamma \vdash \lambda x : A . M : A \supset B$}
    \end{prooftree}

    Otherwise a rule such as the following would not give you
    a unique type.
    \begin{prooftree}
      \AXC{$x:A \in \Gamma$}
      \UIC{$\Gamma \vdash x : A$}
    \end{prooftree}
    \paragraph{Example of substitution} What does this mean?
    \\ $[u/w] (\lambda u.w u) \neq \lambda u. u u$
    \\ You cannot introduce a new variable with the same name as an
    existing one, this will have completely different meaning than you
    intended.
    \\ Solution: $[u/w](\lambda y: w
    u)\stackrel{\alpha}{=}[u/w](\lambda u'. w u') = \lambda u'. u u'$

    Let's assume that $u : T \supset A$.
    \\ $[u/w](\underbrace{\lambda u : T. \ w \ u}_{\text{well-typed, $T
        \supset A$}}) = \lambda u : T. \ \underline{u} \ u$? This is
    ill-typed!
    \subsection{Restatement of Definitions Using Context}
    \paragraph{Weakening} If $\Gamma \vdash M:A$ then $\Gamma, \Gamma'
    \vdash M:A$
    \paragraph{Substitution} If $\Gamma, x : a , \Gamma' \vdash M : B$
    and $\Gamma \vdash N : A$ then $\Gamma, \Gamma' [N/x] M : B$

    How do we prove this? Proof by structural on $\Gamma, x: A,
    \Gamma' \vdash M : B$

    First we must consider each rule that could have been used to derive
    $M : B$.

    Base case would be T, trivially true because there is nothing to
    substitute.

    \subparagraph{Definition of substitution}
    ~\\$[N/x]M = M'$, $[N/x] x = N$. Replace the "free" occurence of
    $x$ in $M$ with $N$
    
    \subparagraph{Case}
    \AXC{$\mathcal{D}'$}
    \noLine
    \UIC{$\Gamma, x:A, \Gamma' \vdash M : C \land D$}
    \RL{$\land$ E$_l$}
    \UIC{$\Gamma, x:A,\Gamma' \vdash fst\ M : C$}
    \DP
    \\ $\Gamma, \Gamma ' \vdash [N/x] M : C\land D$ by IH
    \\ $\Gamma, \Gamma ' \vdash fst\ ([N/x]M) : C$ by $\land$E$_l$
    \\$\Gamma, \Gamma' \vdash [N/x](fst \ M) : C$ by definition of substitution
    \subparagraph{Case}
    \AXC{$\mathcal{D}_1$}
    \noLine
    \UIC{$\Gamma, x:A, \Gamma' \vdash M_1 : D \supset C $}
    
    \AXC{$\mathcal{D}_2$}
    \noLine
    \UIC{$\Gamma, x:A, \Gamma' \vdash M_2 : D$}
    \RL{$\supset$ E}
    \BIC{$\Gamma, x:A,\Gamma' \vdash M_1 \ M_2 : C$}
    \DP
    \\ $\Gamma, \Gamma ' \vdash [N/x] M_1 : D \supset C$ by IH ($\mathcal{D}_1$)
    \\ $\Gamma, \Gamma ' \vdash [N/x] M_2 : D$ by IH ($\mathcal{D}_2$)
    \\$\Gamma, \Gamma' \vdash [N/x]M_1 \ [N/x]M_2 : C$ by $\supset$ E
    \\ $\Gamma, \Gamma' \vdash [N/x](M_1\ M_2) : C$

    The more interesting case is with variables:
    \subparagraph{Case}
    \AXC{$x: A \in (\Gamma, x : A, \Gamma')$}
    
    \UIC{$\Gamma, x : A, \Gamma' \vdash x : A$}
    \DP
    \\ $\Gamma \vdash N.A$ by assumption
    \\ $\Gamma, \Gamma' \vdash N : A$ by weakening
    \\ $\Gamma, \Gamma' \vdash [N/x]x . A$ by substitution definition
    \subparagraph{Case}
    \AXC{$y: B \in (\Gamma, x : A, \Gamma')$}
    \AXC{$x \neq y$}
    
    \BIC{$\Gamma, x : A, \Gamma' \vdash y : B$}
    \DP
    \\ $y:B \in (\Gamma, \Gamma')$
    \\ $\Gamma, \Gamma' \vdash y : B$ by variable
    \subparagraph{Case}
    \AXC{$\Gamma, x : A, \Gamma', y:B \vdash M:C$}
    
    \UIC{$\Gamma, x : A, \Gamma' \vdash \lambda y : B. N:B\supset C$}
    \DP
    \\ $\Gamma, \Gamma', y:B \vdash [N/x] M:C$ by IH.
    \\ $\Gamma, \Gamma', \lambda y : B . [N/x] M:C$ by $\supset$ I 
    \\ $\Gamma \vdash N : A$ by assumption (i.e any var in $N$ is in
    $\Gamma$). $y$ does not occur in $N$
    \\ $\Gamma, \Gamma ' \vdash [N/x] (\lambda y:B.M) : B \supset C$
    by substitution definition
    \section{01/24/19}
    \subsection{More on Proof Terms}
    Last class we saw:
    \\ Prop/Types $A,B:= T \mid \perp \mid A \land B \mid A \supset B
    \mid A \lor B$
    \\ Terms $M,N := \langle  \rangle \mid abort^c \ M \mid \langle
    M,N \rangle \mid fst\ M \mid snd \ M \mid \lambda x . A . M \mid M
    \ N \mid inl^B \ M \mid inr^A \ B \mid (case \ M \ of \ inl \ x
    \implies N_1 \mid inr\ y \implies N_2)$

    We can think of $M:A$ iff $A$ true.
    \paragraph{Warm-up}
    \begin{center}
      \begin{tabular}{l l}
        \textbf{Program} & \textbf{Proposition}
        \\ $\lambda x : A . \lambda y: B. \langle x,y \rangle$ & $A \supset B \supset (A \land B)$
        \\ $\lambda x : A \supset B  \land B \supset C$ & $(A \subset B \land B \supset C) \supset A \supset C$
        \\ ~\hspace{5 pt} $\lambda y: A.(snd\ x)\underbrace{(\underbrace{(fst\ x)}_{A \supset B} y)}_{B}$
        \\ $\lambda x : A \lor B. \lambda y: C$& $(A \lor B) \supset C \supset (B \lor A) \land C$
        \\ ~\hspace{5 pt} $\langle case \ of \ inl \ a \implies inr\ a \mid inr\ b \implies inl\ b,y  \rangle$
      \end{tabular}
    \end{center}
      \paragraph{Reminder}
      \begin{tabular}{l l}
        Prop & Type
        \\ $T$ & unit
        \\ $A \land B$ & $A * B$
        \\ $A \supset B$ & $A \rightarrow B$
        \\ $ A \lor B$ & $A + B$
      \end{tabular}
      The $+$ is usually hidden in programming languages,
      i.e. \texttt{type int\_or\_string = Int of int | Str of string}
      is actually \texttt{Int + String}.
    \begin{center}
      \begin{tabular}{l l}
        \textbf{Proposition} & \textbf{Program}
        \\ $A \supset A$ (has many programs) & $\lambda x:A.x$ \hspace{10 pt}normal/``canonical form''
        \\ Programs on the right are syntactically different & $\lambda x : A . (\lambda y: A . y) x$
        \\ & $\lambda x : A . fst ((\lambda y:A \land A . y) \langle x,x \rangle)$
      \end{tabular}
    \end{center}
    We hope that all of the functions on the right can reduce to the
    normal form.

    If $\Gamma \vdash M : A$ and $M \implies M'$ then $\Gamma \vdash
    M' : A$ \} Subject Reduction/Type Preservation

    By induction (case analysis) on $M \implies M'$
    \subparagraph{Case} $fst \langle M,N \rangle \implies M$
    \\\begin{tabular}{l l}
    $\Gamma \vdash fst\ \langle M,N \rangle : A$ & by assumption
    \\ $\Gamma \vdash \langle M,N \rangle : A \land B$ & by \underline{inversion} on
    $\land$ E$_l$
    \end{tabular}

    Note the inversion rule tells us:
    \begin{prooftree}
      \AXC{$M : A \land B$}
      \RL{$\land$ E$_l$}
      \UIC{$fst\ M : A$}
    \end{prooftree}
    Inversion Lemma: If $fst\ M : A$ then $M:A \land B$. This is
    obvious in this system because there is only one rule. If there
    was another rule that we could use, then we'd have to prove that
    it came from this inversion rule.
    \\\begin{tabular}{l l}
    $\Gamma \vdash M : A$ & by \underline{inversion} of $\land I$
    \end{tabular}

    The concept of \underline{inversion} is very important, we want to
    know where the term comes from.
    \subparagraph{Case} $(\lambda x : A.M) N \implies [N/x] M$
    \\\begin{tabular}{l l}
    $\Gamma \vdash (\lambda x : A . M) N : B$ & by assumption
    \\ $\Gamma \vdash \lambda x: A.M : A \supset B \ \Gamma \vdash N :
    A$ & by inversion on $\supset$ E
    \\ $\Gamma, x : A \vdash M : B$ & by inversion on $\supset$ I
    \\ $\Gamma \vdash [N/x]M:B$ & by substitution lemma (on above line
    and $\Gamma \vdash N:A$)
    \end{tabular}
    \subparagraph{Case} $case\ (inl^B \ M) \ of \ inl\ x \implies N_1
    \mid inr\ y \implies N_2 \implies [M/x] N_1$
    \\\begin{tabular}{l l}
    $\Gamma \vdash case\ (inl^B \ M) \ of \ inl\ x \implies N_1
        \mid inr\ y \implies N_2 : C $ & by assumption
        \\ $\Gamma \vdash inl^B \ M : A \lor B$ & by inversion $\lor$ E
        \\ $\Gamma, x:A \vdash N_1 : C$
        \\ $\Gamma, x:B \vdash N_2 : C$
        \\ $\Gamma \vdash M.A : C$ & by inversion $\lor$ I$_l$
        \\ $\Gamma \vdash [M/x]N_1 : C$ & by substitution
      \end{tabular}
      \subparagraph{Case} \AXC{$M_1 \implies M'$}
      \UIC{$M_1 \ M_2 \implies M_1' M_2$}
      \DP
      \\
      \begin{tabular}{l l}
        $\Gamma \vdash M_1 \ M_2 : B$& by assumption
        \\ $\Gamma \vdash M_1 : A \supset B$ and $\Gamma \vdash M_2 : A$ & by inversion $\supset$E
        \\ $\Gamma \vdash M_1' : A \supset B$ & by IH
        \\ $\Gamma \vdash M_1' M_1 : B$ & by $\supset$ E
      \end{tabular}
      The last step is forward reasoning instead of backward reasoning
      with inversions. Basically show what your case gives you and
      then apply IH to get what you want.
      \subparagraph{Case}
      \AXC{$M \implies M'$}
      \UIC{$\lambda x : A.M \implies \lambda x: A.M'$}
      \DP
      \\\begin{tabular}{l l}
        $\Gamma \vdash \lambda x : A . M : A \supset B$& by assumption
          \\ $\Gamma, x : A \vdash M:B$ & by inversion on $\supset$ I
          \\ $\Gamma, x:A \vdash M' : B$ & by IH
          \\ $\Gamma \vdash \lambda x : A . M' : A \supset B$ & by $\supset$ I
        \end{tabular}

      Note that in trying to reduce $fst\ ((\lambda y:A \land A. y)
      \langle x,x \rangle)$, we will need to step twice:
      \\ $\implies \lambda x : A . fst \langle x,x \rangle$
      \\ $\implies \lambda x : A . x$
      \\ But so far we are only stepping once.
      \paragraph{Can we prove the opposite?}
      If $\Gamma \vdash M' : A$ and $M \implies M'$ then $\Gamma
      \vdash M : A$
      \subparagraph{Case} $fst \langle M,N \rangle \implies M$
      \\\begin{tabular}{l l}
          $\Gamma \vdash M :A$& by assumption
          \\ $\Gamma \vdash N : B$ & How to show this?
          \\ $\Gamma \vdash \langle M,N \rangle : A \land B$
          \\ $\Gamma \vdash fst \ \langle M,N \rangle : A$ & To show
        \end{tabular}
        Cannot prove this syntactically right now.
        \paragraph{Multi Step} Want to step multiple times. $M
        \implies^* M'$, meaning $M$ steps in more than one step.
        \begin{prooftree}
          \AXC{}
          \RL{refl(ectivity)}
          \UIC{$M \implies^* M$}
        \end{prooftree}
        \begin{prooftree}
          \AXC{$M \implies^* K$}
          \AXC{$K \implies^* N$}
          \RL{Trans(itivity)}
          \BIC{$M \implies^* N$}
        \end{prooftree}
        \begin{prooftree}
          \AXC{$M \implies N$}
          \RL{one-step}
          \UIC{$M \implies^* N$}
        \end{prooftree}
        \subsection{Normal Form}
        What is a normal form when no reduction is possible anymore?
        \\ $\lambda :A \supset B.\lambda y : A . x \ y$ is a normal
        form
        \\ So is $\lambda x : (A \supset A)\supset C . x \underbrace{(\lambda y: A
          . y)}_{A \supset A}$
        \\ Basically, you can no longer reduce the expression.
        \paragraph{Normal Form} $m,n : = \lambda x:A.m \mid r$
        \paragraph{Neutral Form} $r : = x \mid r \ m \mid fst\ r \mid
        snd\ r$
        \paragraph{Questions}
        \begin{enumerate}
        \item Can we always reach a normal form? (Does reduction
          terminate?)
        \item Can we change the proof that correspond to the normal
          forms? ``Normal Proof'' (without any detours)
        \item Is there a unique normal form that can be computed?
          \\ If $M \implies^* N_1$ and $M \implies^* N_2$ then $N_1 = N_2$
        \end{enumerate}
        Will look at 1 and 2 before the midterm.
      \end{document}