\documentclass[12pt]{article}
\usepackage{fancyhdr}
\usepackage[margin=1 in,headheight=20pt]{geometry}
\usepackage{setspace}
\usepackage{amsmath}
\usepackage{amsthm}
\usepackage{amssymb}
\usepackage{enumerate}
\usepackage{relsize}
\usepackage{lastpage}
\allowdisplaybreaks

\theoremstyle{plain} 
\newtheorem*{thm}{Theorem}

\pagestyle{fancy}
\lhead{COMP 302-001}
\chead{practice.ml Induction Proof}
\rhead{\today
	\\ LORE, JULIAN}
\cfoot{Page \thepage \ of \pageref{LastPage}}

\begin{document}
\onehalfspacing
\begin{thm}
  For all lists \texttt{l}, \texttt{even\_parity l} $=$ \texttt{even\_parity\_tr l}.
\end{thm}
\begin{proof}
  By structural induction on \texttt{l}.
  \begin{itemize}
  \item \textbf{Base case}: \texttt{l = []}
    \begin{align*}
      \texttt{even\_parity l} &= \texttt{even\_parity []} &
      \\ & =
           \texttt{false} & \text{By definition of \texttt              {even\_parity}}
      \\ & = \texttt{parity false []} & \text{By                           definition of \texttt{parity}}
      \\ & =
           \texttt{even\_parity\_tr
           []} & \text{By definition of \texttt{even\_parity\_tr}}
      \\ & = \texttt{even\_parity\_tr l}
    \end{align*}
  \item \textbf{Step}: \texttt{l} $=$ \texttt{x ::\ xs} for some element
    \texttt{x} and list \texttt{xs}.
    \\ \textbf{Inductive Hypothesis}: \texttt{even\_parity xs} $=$
    \texttt{even\_parity\_tr xs}
    \begin{itemize}
    \item Case 1. \texttt{x} $=$ \texttt{true}
      \begin{align*}
        & \texttt{even\_parity\_tr l}
        \\ & = \texttt{even\_parity\_tr true ::\ xs}
        \\ & = \texttt{parity false true ::\ xs} & \text{By              definition of \texttt{even\_parity\_tr}}
        \\ & = \texttt{parity (false <> true) xs} & \text{By
                                                    definition of \texttt{parity}}
        \\ & = \texttt{parity true xs} & \text{By definition of $\oplus$}
        \\ & = \texttt{not (not(parity true xs))} & \text{By definition
                                                  of not}
        \\  (*) & = \texttt{not (parity false xs)} & \text{Since
                                                 \texttt{parity false
                                                 l} $=$ \texttt{not parity true l}}
        \\ & = \texttt{not (even\_parity\_tr xs)} & \text{By
                                                    definition of \texttt{even\_parity\_tr}}
        \\ & = \texttt{not (even\_parity xs)} & \text{By IH}
        \\ & = \texttt{even\_parity true ::\ xs} & \text{By definition
                                                   of \texttt{even\_parity}}
      \end{align*}
    \item Case 2. \texttt{x} $=$ \texttt{false}.
      \begin{align*}
        & \texttt{even\_parity\_tr l}
        \\ & = \texttt{even\_parity\_tr false ::\ xs}
        \\ & = \texttt{parity false false ::\ xs} & \text{By
                                                    definition of \texttt{even\_parity\_tr}}
        \\ & = \texttt{parity (false <> false) xs} & \text{By
                                                     definition of \texttt{parity}}
        \\ & = \texttt{parity false xs} & \text{By definition of $\oplus$}
        \\ & = \texttt{even\_parity xs} & \text{By IH}
        \\ & = \texttt{even\_parity false ::\ xs} & \text{By
                                                    definition of \texttt{even\_parity}}
      \end{align*}
    \end{itemize}
  \end{itemize}
  \textit{Step (*) may not be correct/may require more expansion.}
\end{proof}
\end{document}